examples/layeredeffects/LowParseWriters.LowParse.fsti
@@ -1,0 +1,181 @@
+module LowParseWriters.LowParse
+
+module HS = FStar.HyperStack
+module B = LowStar.Buffer
+module U8 = FStar.UInt8
+module U32 = FStar.UInt32
+module HST = FStar.HyperStack.ST
+
+type u8 : Type0 = U8.t
+
+val parser' (t: Type0) : Type0
+let parser : Type u#1 = (t: Type0 & parser' t)
+
+val valid_pos
+  (p: parser)
+  (h: HS.mem)
+  (b: B.buffer U8.t)
+  (pos: U32.t)
+  (pos' : U32.t)
+: GTot Type0
+
+val valid_pos_post
+  (p: parser)
+  (h: HS.mem)
+  (b: B.buffer U8.t)
+  (pos: U32.t)
+  (pos' : U32.t)
+: Lemma
+  (requires (valid_pos p h b pos pos'))
+  (ensures (
+    B.live h b /\
+    U32.v pos <= U32.v pos' /\
+    U32.v pos' <= B.length b
+  ))
+  [SMTPat (valid_pos p h b pos pos')]
+
+val contents
+  (p: parser)
+  (h: HS.mem)
+  (b: B.buffer U8.t)
+  (pos: U32.t)
+  (pos' : U32.t)
+: Ghost (dfst p)
+  (requires (valid_pos p h b pos pos'))
+  (ensures (fun _ -> True))
+
+val size
+  (p: parser)
+  (x: dfst p)
+: GTot nat
+
+val contents_size
+  (p: parser)
+  (h: HS.mem)
+  (b: B.buffer U8.t)
+  (pos: U32.t)
+  (pos' : U32.t)
+: Lemma
+  (requires (valid_pos p h b pos pos'))
+  (ensures (
+    valid_pos p h b pos pos' /\
+    size p (contents p h b pos pos') == U32.v pos' - U32.v pos
+  ))
+  [SMTPat (contents p h b pos pos')]
+
+val emp' : parser' unit
+
+let emp : parser = (| unit, emp' |)
+
+val valid_emp
+  (h: HS.mem)
+  (b: B.buffer u8)
+  (pos: U32.t)
+  (pos' : U32.t)
+: Lemma
+  (
+    valid_pos emp h b pos pos' <==> (
+    B.live h b /\
+    U32.v pos <= B.length b /\
+    U32.v pos' == U32.v pos
+  ))
+  [SMTPat (valid_pos emp h b pos pos')]
+
+val size_emp : squash (size emp () == 0)
+
+val star' (#t1 #t2: Type) (p1: parser' t1) (p2: parser' t2) : Tot (parser' (t1 & t2))
+
+let star (p1 p2: parser) : Tot parser = (| (dfst p1 & dfst p2), star' (dsnd p1) (dsnd p2) |)
+
+val valid_star
+  (p1 p2: parser)
+  (h: HS.mem)
+  (b: B.buffer U8.t)
+  (pos1 pos2 pos3: U32.t)
+: Lemma
+  (requires (
+    valid_pos p1 h b pos1 pos2 /\
+    valid_pos p2 h b pos2 pos3
+  ))
+  (ensures (
+    valid_pos p1 h b pos1 pos2 /\
+    valid_pos p2 h b pos2 pos3 /\
+    valid_pos (p1 `star` p2) h b pos1 pos3 /\
+    contents (p1 `star` p2) h b pos1 pos3 == (contents p1 h b pos1 pos2, contents p2 h b pos2 pos3)
+  ))
+
+val size_star
+  (p1 p2: parser)
+  (x1: dfst p1)
+  (x2: dfst p2)
+: Lemma
+  (size (p1 `star` p2) (x1, x2) == size p1 x1 + size p2 x2)
+  [SMTPat (size (p1 `star` p2) (x1, x2))]
+
+val valid_frame
+  (p: parser)
+  (h: HS.mem)
+  (b: B.buffer U8.t)
+  (pos: U32.t)
+  (pos' : U32.t)
+  (l: B.loc)
+  (h' : HS.mem)
+: Lemma
+  (requires (
+    valid_pos p h b pos pos' /\
+    B.modifies l h h' /\
+    B.loc_disjoint l (B.loc_buffer_from_to b pos pos')
+  ))
+  (ensures (
+    valid_pos p h b pos pos' /\
+    valid_pos p h' b pos pos' /\
+    contents p h' b pos pos' == contents p h b pos pos'
+  ))
+
+val valid_gsub
+  (p: parser)
+  (h: HS.mem)
+  (b: B.buffer U8.t)
+  (pos0 pos1 pos2: U32.t)
+  (len: U32.t)
+: Lemma
+  (requires (
+    U32.v pos0 + U32.v len <= B.length b /\
+    valid_pos p h (B.gsub b pos0 len) pos1 pos2
+  ))
+  (ensures (
+    U32.v pos0 + U32.v pos2 <= B.length b /\
+    valid_pos p h (B.gsub b pos0 len) pos1 pos2 /\
+    valid_pos p h b (pos0 `U32.add` pos1) (pos0 `U32.add` pos2) /\
+    contents p h b (pos0 `U32.add` pos1) (pos0 `U32.add` pos2) == contents p h (B.gsub b pos0 len) pos1 pos2
+  ))
+  [SMTPat (valid_pos p h (B.gsub b pos0 len) pos1 pos2)]
+
+val parse_u32' : parser' U32.t
+
+let parse_u32 : parser = (| U32.t , parse_u32' |)
+
+inline_for_extraction
+let leaf_writer
+  (p: parser)
+: Tot Type
+=
+  (b: B.buffer U8.t) ->
+  (len: U32.t { len == B.len b }) ->
+  (x: dfst p) ->
+  HST.Stack (option U32.t)
+  (requires (fun h -> B.live h b))
+  (ensures (fun h res h' ->
+    match res with
+    | None ->
+      B.modifies (B.loc_buffer b) h h' /\
+      size p x > B.length b
+    | Some xlen ->
+      U32.v xlen <= B.length b /\
+      B.modifies (B.loc_buffer_from_to b 0ul xlen) h h' /\
+      valid_pos p h' b 0ul xlen /\
+      contents p h' b 0ul xlen == x /\
+      size p x == U32.v xlen
+  ))  
+
+val write_u32 : leaf_writer parse_u32
